src/FlattenedComp.v
@@ -1,0 +1,79 @@
+Require Import Common Monads.
+Require Switched Flattened.
+
+Module S := Switched.
+Module F := Flattened.
+
+Section compile.
+
+  Open Scope state_monad.
+
+  Definition compiler_monad A := state nat A.
+
+  Definition fresh : compiler_monad nat :=
+    get >>= fun n => put (S n) >>= fun _ => ret_state n.
+
+  Fixpoint sequence (l : list F.stmt) : F.stmt :=
+    match l with
+    | [] => F.Skip
+    | s :: l' => F.Seq s (sequence l')
+    end.
+
+  Definition compile' (e : S.expr) : compiler_monad (F.stmt * F.expr) :=
+    let fix go (e : S.expr) : compiler_monad (F.stmt * F.expr) :=
+        let fix go_list (l : list S.expr) : compiler_monad (list (F.stmt * F.expr)) :=
+            match l with
+            | [] => ret_state []
+            | e :: l' => cons <$> go e <*> go_list l'
+            end
+        in
+        match e with
+        | S.Arg => ret_state (F.Skip, F.Arg)
+        | S.UpVar n => ret_state (F.Skip, F.Deref F.Self n)
+        | S.Deref e' n =>
+          go e' >>= fun p =>
+          let (s', e') := p in
+          ret_state (s', F.Deref e' n)
+        | S.Call f a =>
+          go f >>= fun pf =>
+          let (sf, f) := pf in
+          go a >>= fun pa =>
+          let (sa, a) := pa in
+          fresh >>= fun dst =>
+          ret_state (F.Seq sf (F.Seq sa (F.Call dst f a)), F.Temp dst)
+        | S.Constr tag args =>
+          go_list args >>= fun psargs =>
+          let (sargs, args) := split psargs in
+          fresh >>= fun dst =>
+          ret_state (F.Seq (sequence sargs) (F.MakeConstr dst tag args), F.Temp dst)
+        | S.Switch cases target =>
+          go_list cases >>= fun pscases =>
+          go target >>= fun ptarget =>
+          let (starget, target) := ptarget in
+          fresh >>= fun dst =>
+          ret_state (F.Seq starget (F.Switch (map (fun p => let (s, e) := p : _ * _ in F.Seq s (F.Assign dst e)) pscases) target), F.Temp dst)
+        | S.Close fn args =>
+          go_list args >>= fun psargs =>
+          let (sargs, args) := split psargs in
+          fresh >>= fun dst =>
+          ret_state (F.Seq (sequence sargs) (F.MakeClose dst fn args), F.Temp dst)
+        end
+    in go e.
+
+  Definition compile (e : S.expr) : F.stmt * F.expr := fst (compile' e 0).
+
+  Fixpoint compile_env' (l : list S.expr) : compiler_monad (list (F.stmt * F.expr)) :=
+    match l with
+    | [] => ret_state []
+    | e :: l' => cons <$> compile' e <*> compile_env' l'
+    end.
+
+  Definition compile_env (l : list S.expr) : list (F.stmt * F.expr) := fst (compile_env' l 0).
+
+  Definition compile_prog (p : S.expr * list S.expr) :
+    list (F.stmt * F.expr) * nat :=
+    let (e, env) := p in (compile_env (env ++ [e]), length env).
+
+End compile.
+
+Eval compute in compile_prog Switched.add_prog2.
